symbolic/forward.v
@@ -7,12 +7,15 @@ Require Import common.common.
 Require Import concrete.concrete.
 Require Import concrete.exec.
 Require Import symbolic.symbolic.
+Require Import symbolic.exec.
 Require Import symbolic.rules.
 Require Import symbolic.refinement_common.
 
 Open Scope nat_scope.
 
 Set Implicit Arguments.
+Unset Strict Implicit.
+Unset Printing Implicit Defensive.
 
 Import ListNotations.
 
@@ -26,7 +29,7 @@ Context {mt : machine_types}
         {ops : machine_ops mt}
         {opss : machine_ops_spec ops}
         {sp : Symbolic.params}
-        {e : forall k, encodable mt (Symbolic.ttypes k)}
+        {e : encodable mt Symbolic.ttypes}
         {ki : kernel_invariant}
         {table : list (Symbolic.syscall mt)}
         {kcc : kernel_code_correctness ki table}.
@@ -46,128 +49,191 @@ Hint Unfold Concrete.next_state_pc.
 Hint Unfold Concrete.next_state.
 Hint Unfold Concrete.miss_state.
 
-Let in_kernel_user k t : Concrete.is_kernel_tag (@encode _ _ (e k) (USER t)) = false.
-Proof.
-  unfold Concrete.is_kernel_tag.
-  erewrite encode_kernel_tag.
-  now erewrite eq_tag_eq_word.
-Qed.
-
 Lemma user_mem_unchanged_refine_memory amem cmem cmem' :
   refine_memory amem cmem ->
   user_mem_unchanged cmem cmem' ->
   refine_memory amem cmem'.
 Proof.
-  intros REF USERMEM addr x t.
-  rewrite <- (USERMEM addr).
-  apply REF.
+  move=> [REF1 REF2] USERMEM.
+  split.
+  - move=> w x ctg atg DEC GET.
+    move: (USERMEM w x ctg atg) (conj GET DEC) => H /H {H} {GET DEC} [GET DEC].
+    by eauto.
+  - move=> w x atg /REF2 [ctg DEC GET].
+    move: (USERMEM w x ctg atg) (conj GET DEC) => H /H {H} {GET DEC} [GET DEC].
+    by eauto.
 Qed.
 
-Lemma user_regs_unchanged_refine_registers areg creg creg' :
-  refine_registers areg creg ->
-  user_regs_unchanged creg creg' ->
-  refine_registers areg creg'.
+Lemma user_regs_unchanged_refine_registers areg creg creg' cmem cmem' :
+  refine_registers areg creg cmem ->
+  user_regs_unchanged creg creg' cmem cmem' ->
+  refine_registers areg creg' cmem'.
 Proof.
-  intros REF USERREG r x t.
-  rewrite <- (USERREG r).
-  apply REF.
+  move=> [REF1 REF2] USERREGS.
+  split.
+  - move=> r x ctg atg DEC GET.
+    move: (USERREGS r x ctg atg) (conj GET DEC) => H /H {USERREGS H GET DEC} [GET DEC].
+    by eauto.
+  - move=> r x atg /REF2 [ctg DEC GET].
+    move: (USERREGS r x ctg atg) (conj GET DEC) => H /H {USERREGS H GET DEC} [GET DEC].
+    by eauto.
 Qed.
 
-Ltac match_data :=
-  repeat match goal with
-  | H : PartMaps.get ?amem ?addr = Some ?w,
-    REFM : refine_memory ?amem ?cmem |- _ =>
+Ltac failwith message :=
+  let op := current_instr_opcode in
+  fail 1000 message op.
+
+Ltac check_conv t1 t2 :=
+  let e := constr:(erefl t1 : t1 = t2) in idtac.
+
+Ltac match_mem_get REF sst cst :=
+  match goal with
+  | GET : PartMaps.get ?smem ?addr = Some ?w@?t |- _ =>
+    check_conv smem (Symbolic.mem sst);
     match goal with
-    | _ : PartMaps.get cmem addr = _ |- _ => fail 1
+    | _ : PartMaps.get ?cmem addr = _ |- _ => check_conv cmem (Concrete.mem cst); fail 1
     | |- _ => idtac
     end;
-    apply REFM in H
+    first [ have [? ? ?] := proj2 (rs_refm REF) _ _ _ GET
+          | failwith "match_mem" ]
+  end.
 
-  | GET : PartMaps.get ?mem1 ?addr = Some ?x@(encode (USER ?t)),
+Ltac match_mem_upd REF sst cst :=
+  match goal with
+  | UPD : PartMaps.upd ?smem ?addr ?w@?t = Some ?smem',
+    DEC : decode Symbolic.M ?cmem ?ct = Some (USER ?t) |- _ =>
+    check_conv smem (Symbolic.mem sst);
+    match goal with
+    | _ : refine_memory smem' ?cmem',
+      _ : PartMaps.upd cmem ?addr _ = Some ?cmem' |- _ => fail 1
+    | |- _ => idtac
+    end;
+    first [ let cmem' := fresh "cmem'" in
+            let UPD' := fresh "UPD'" in
+            let REFR' := fresh "REFR'" in
+            let REFM' := fresh "REFM'" in
+            let CACHE' := fresh "CACHE'" in
+            destruct (refine_memory_upd' (rs_cache REF) (rs_refr REF) (rs_refm REF) UPD DEC)
+              as (cmem' & [UPD' CACHE' REFR' REFM'])
+          | failwith "match_mem_upd" ]
+  end.
+
+Ltac match_mem_unchanged REF sst cst :=
+  match goal with
+  | USERMEM : user_mem_unchanged ?cmem ?cmem' |- _ =>
+    check_conv cmem (Concrete.mem cst);
+    match goal with
+    | _ : refine_memory ?smem cmem' |- _ => check_conv smem (Symbolic.mem sst); fail 1
+    | |- _ => idtac
+    end;
+    first [ pose proof (user_mem_unchanged_refine_memory (rs_refm REF) USERMEM)
+          | failwith "match_mem_unchanged" ]
+  end.
+
+Ltac match_mem_unchanged_tags :=
+  match goal with
+  | GET : PartMaps.get ?mem1 ?addr = Some ?x@?ct,
+    DEC : decode Symbolic.M ?mem1 ?ct = Some (USER ?t),
     USERMEM : user_mem_unchanged ?mem1 ?mem2 |- _ =>
     match goal with
     | _ : PartMaps.get mem2 addr = _ |- _ => fail 1
     | |- _ => idtac
     end;
-    assert (PartMaps.get mem2 addr = Some x@(encode (USER t)));
-    try solve [eapply USERMEM; assumption]
+    first [ have [? ?] : (PartMaps.get mem2 addr = Some x@ct /\
+                          decode Symbolic.M mem2 ct = Some (USER t))
+                          by apply/USERMEM; eauto
+          | failwith "match_mem_unchanged_tags" ]
+  end.
 
-  | H : PartMaps.upd ?amem ?addr _ = Some ?amem',
-    REFM : refine_memory ?amem ?cmem |- _ =>
+Ltac match_reg_get REF sst cst :=
+  match goal with
+  | GET : PartMaps.get ?sregs ?r = Some ?w@?t |- _ =>
+    check_conv sregs (Symbolic.regs sst);
     match goal with
-    | _ : refine_memory amem' ?cmem',
-      _ : PartMaps.upd cmem ?addr _ = Some ?cmem'|- _ => fail 1
+    | _ : PartMaps.get ?cregs r = Some _ |- _ => check_conv cregs (Concrete.regs cst); fail 1
     | |- _ => idtac
     end;
-    let cmem' := fresh "cmem'" in
-    let UPD' := fresh "UPD'" in
-    let REFM' := fresh "REFM'" in
-    destruct (refine_memory_upd' _ _ _ REFM H) as (cmem' & UPD' & REFM')
+    first [ destruct (proj2 (rs_refr REF) _ _ _ GET) as [? ? ?]
+          | failwith "match_reg_get" ]
+  end.
 
-  | H : PartMaps.get ?aregs ?r = Some _,
-    REFR : refine_registers ?aregs ?cregs |- _ =>
-    apply REFR in H
-
-  | UPD : PartMaps.upd ?aregs ?r _ = Some ?aregs',
-    REFR : refine_registers ?aregs ?cregs |- _ =>
+Ltac match_reg_upd REF sst cst :=
+  match goal with
+  | UPD : PartMaps.upd ?sregs ?r ?w@?t = Some ?sregs',
+    DEC : decode Symbolic.R ?cmem ?ct = Some (USER ?t) |- _ =>
+    check_conv sregs (Symbolic.regs sst);
     match goal with
-    | _ : refine_registers aregs' ?cregs',
-      _ : PartMaps.upd cregs r _ = Some ?cregs'|- _ => fail 1
+    | _ : refine_registers sregs' ?cregs' cmem,
+      _ : PartMaps.upd _ r _ = Some ?cregs' |- _ => fail 1
     | |- _ => idtac
     end;
     let cregs' := fresh "cregs'" in
     let UPD' := fresh "UPD'" in
     let REFR' := fresh "REFR'" in
-    destruct (refine_registers_upd' _ _ _ REFR UPD) as (cregs' & UPD' & REFR')
+    first [ destruct (refine_registers_upd' (rs_refr REF) UPD DEC) as [cregs' UPD' REFR']
+          | failwith "match_reg_upd" ]
+  end.
 
-  | REFM : refine_memory ?smem ?cmem,
-    USERMEM : user_mem_unchanged ?cmem ?cmem' |- _ =>
+Ltac match_reg_unchanged REF sst cst :=
+  match goal with
+  | USERREGS : user_regs_unchanged ?cregs ?cregs' |- _ =>
+    check_conv cregs (Concrete.regs cst);
     match goal with
-    | _ : refine_memory smem cmem' |- _ => fail 1
+    | _ : refine_registers ?sregs cregs' |- _ => check_conv sregs (Symbolic.regs sst); fail 1
     | |- _ => idtac
     end;
-    pose proof (user_mem_unchanged_refine_memory REFM USERMEM)
+    first [ pose proof (user_regs_unchanged_refine_registers (rs_refr REF) USERREGS)
+          | failwith "match_data 7" ]
 
-  | REFR : refine_registers ?sregs ?cregs,
-    USERREGS : user_regs_unchanged ?cregs ?cregs' |- _ =>
-    match goal with
-    | _ : refine_registers sregs cregs' |- _ => fail 1
-    | |- _ => idtac
-    end;
-    pose proof (user_regs_unchanged_refine_registers REFR USERREGS)
+  end.
 
+Ltac match_data :=
+  match goal with
+  | REF : refine_state _ _ ?sst ?cst |- _ =>
+    repeat first [ match_mem_get REF sst cst
+                 | match_mem_upd REF sst cst
+                 | match_mem_unchanged REF sst cst
+                 | match_mem_unchanged_tags
+                 | match_reg_get REF sst cst
+                 | match_reg_upd REF sst cst
+                 | match_reg_unchanged REF sst cst ]
   end.
 
 Ltac user_data_unchanged :=
   match goal with
-  | GET : PartMaps.get ?mem1 ?addr = Some _,
-    USERMEM : user_mem_unchanged ?mem1 ?mem2
-    |- PartMaps.get ?mem2 ?addr = Some _ =>
-    simpl in GET, USERMEM;
-    rewrite <- (USERMEM addr); eassumption
+  | GET : PartMaps.get ?mem1 ?addr = Some ?w@?ct,
+    DEC : decode Symbolic.M ?mem1 ?ct = Some (USER ?t),
+    USERMEM : user_mem_unchanged ?mem1 ?mem2 |- _ =>
+    match goal with
+    | _ : PartMaps.get mem2 addr = Some _ |- _ => fail 1
+    | |- _ => idtac
+    end;
+    first [ destruct (proj1 (USERMEM _ _ _ _) (conj GET DEC)) as [? ?]
+          | failwith "user_data_unchanged 1" ]
 
-  | GET : PartMaps.get ?regs1 ?r = _,
-    USERREGS : user_regs_unchanged ?regs1 ?regs2
-    |- PartMaps.get ?regs2 ?r = _ =>
-    simpl in GET, USERREGS;
-    rewrite <- (USERREGS r); eauto
+  | GET : PartMaps.get ?regs1 ?r = Some ?w@?ct,
+    DEC : decode Symbolic.R ?cmem1 ?ct = Some (USER ?t),
+    USERREGS : user_regs_unchanged ?regs1 ?regs2 ?cmem1 ?cmem2 |- _ =>
+    match goal with
+    | _ : PartMaps.get regs2 r = Some _ |- _ => fail 1
+    | |- _ => idtac
+    end;
+    first [ destruct (proj1 (USERREGS _ _ _ _) (conj GET DEC)) as [? ?]
+          | failwith "user_data_unchanged 2" ]
   end.
 
 Lemma no_syscall_no_entry_point mem addr t :
   wf_entry_points table mem ->
   Symbolic.get_syscall table addr = None ->
   ~~ match PartMaps.get mem addr with
-     | Some i@it => (is_nop i) && (it == @encode _ _ (e Symbolic.M) (ENTRY t))
+     | Some i@it => (is_nop i) && (decode Symbolic.M mem it == Some (ENTRY t))
      | None => false
      end.
 Proof.
   intros WF GETSC.
-  destruct (match PartMaps.get mem addr with
-            | Some i@it => (is_nop i) && (it == @encode _ _ (e Symbolic.M) (ENTRY t))
-            | None => false
-            end) eqn:E; trivial.
-  apply WF in E.
-  destruct E as [? [? ?]]. congruence.
+  apply/negP=> E.
+  move: (proj2 (WF addr t) E) => [? [? ?]].
+  congruence.
 Qed.
 
 Ltac solve_concrete_step :=
@@ -188,15 +254,9 @@ Ltac solve_concrete_step :=
                          end; match_inv; eauto])
   end.
 
-Ltac destruct_mvec_operands :=
-  repeat match goal with
-  | ts : Vector.t _ 0 |- _ => induction ts using Vector.case0
-  | ts : Vector.t _ (S _) |- _ => induction ts using caseS
-  | ts : Empty_set |- _ => destruct ts
-  end.
-
-Lemma symbolic_handler_concrete_cache cache umvec urvec rvec :
-  cache_correct cache ->
+(*
+Lemma symbolic_handler_concrete_cache cache cmem umvec urvec rvec :
+  cache_correct cache cmem ->
   Symbolic.transfer umvec = Some urvec ->
   Concrete.cache_lookup cache masks (encode_ivec _ (ivec_of_uivec umvec)) = Some rvec ->
   rvec = encode_ovec _ (ovec_of_uovec urvec).
@@ -214,7 +274,9 @@ Proof.
   apply ivec_of_uivec_inj in E1. subst.
   congruence.
 Qed.
+*)
 
+(*
 Lemma symbolic_handler_concrete_handler mvec rvec :
   Symbolic.transfer mvec = Some rvec ->
   ~~ privileged_op (Symbolic.op mvec) ->
@@ -226,9 +288,11 @@ Proof.
              -(lock ivec_of_uivec) ivec_of_uivec_privileged
              (negbTE PRIV) ivec_of_uivecK /= H /=.
 Qed.
+*)
 
-Ltac solve_refine_state :=
-  unfold in_user, word_lift in *; simpl in *;
+
+Ltac solve_refine_state := idtac. (*
+  unfold in_user in *; simpl in *;
   repeat rewrite decodeK; simpl in *;
   try match goal with
   | USERREGS : user_regs_unchanged ?cregs _,
@@ -240,6 +304,7 @@ Ltac solve_refine_state :=
               refine_registers_upd', user_regs_unchanged_refine_registers,
               mvec_in_kernel_user_upd, wf_entry_points_user_upd,
               no_syscall_no_entry_point.
+*)
 
 Ltac analyze_syscall :=
   match goal with
@@ -255,7 +320,7 @@ Ltac analyze_syscall :=
     [apply user_kernel_user_step_weaken; eassumption|solve_refine_state]
   end.
 
-Ltac analyze_cache_miss :=
+Ltac analyze_cache_miss := idtac. (*
   match goal with
   | PC : PartMaps.get ?cmem ?pc = Some ?i@_,
     INST : decode_instr ?i = Some _,
@@ -277,17 +342,67 @@ Ltac analyze_cache_miss :=
     match_data;
     unfold encode_ivec, encode_ovec, ovec_of_uovec in *; simpl in *
   end.
+*)
+
+Ltac find_and_rewrite :=
+  repeat match goal with
+  | H : ?x = _ |- context[?x] =>
+    rewrite H /=
+  end.
+
+Ltac concretize_ivec :=
+  match goal with
+  | TRANS : Symbolic.transfer ?ivec = Some _,
+    REF : refine_state _ _ ?sst ?cst |- _ =>
+    let ivec := eval hnf in ivec in
+    let mvec := match ivec with
+                | Symbolic.mkIVec ?op ?tpc ?ti ?ts =>
+                  let op := match op with
+                            | OP ?op => op
+                            end in
+                  let cti := match goal with
+                             | _ : decode Symbolic.M _ ?cti = Some (USER ti) |- _ => cti
+                             end in
+                  let ct1 := match ts with
+                             | (?t1, _) =>
+                               match goal with
+                               | _ : decode _ _ ?ct1 = Some (USER t1) |- _ => ct1
+                               end
+                             | _ => constr:(@Concrete.TNone mt)
+                             end in
+                  let ct2 := match ts with
+                             | (_, (?t2, _)) =>
+                               match goal with
+                               | _ : decode _ _ ?ct2 = Some (USER t2) |- _ => ct2
+                               end
+                             | _ => constr:(@Concrete.TNone mt)
+                             end in
+                  let ct3 := match ts with
+                             | (_, (_, (?t3, _))) =>
+                               match goal with
+                               | _ : decode _ _ ?ct3 = Some (USER t3) |- _ => ct3
+                               end
+                             | _ => constr:(@Concrete.TNone mt)
+                             end in
+                  constr:(Concrete.mkMVec (op_to_word op) (common.tag (Concrete.pc cst)) cti ct1 ct2 ct3)
+                end in
+    assert (build_cmvec cst = Some mvec /\(* by (rewrite /build_cmvec; find_and_rewrite; reflexivity);*)
+            build_ivec table sst = Some ivec)
+  end.
 
 Ltac analyze_step :=
   match goal with
-  | rvec : _,
-    CACHE : cache_correct ?cache,
-    HANDLER : Symbolic.transfer ?mvec = Some ?rvec |- _ =>
+  | CACHE : refine_state _ _ ?sst ?cst,
+    HANDLER : Symbolic.transfer ?ivec = Some ?ovec |- _ =>
     let trpc := fresh "trpc" in
     let tr   := fresh "tr"   in
-    destruct rvec as [trpc tr]; simpl in tr;
-    let cmvec := constr:(encode_ivec e (ivec_of_uivec mvec)) in
-    destruct (Concrete.cache_lookup cache masks cmvec) as [rvec' | ] eqn:LOOKUP;
+    let ctrpc := fresh "ctrpc" in
+    let ctr := fresh "ctr" in
+    let rvec := fresh "rvec" in
+    try simpl in ovec;
+    destruct ovec as [trpc tr]; simpl in tr; idtac (*
+    let cmvec := concretize_ivec in
+    destruct (Concrete.cache_lookup cache masks cmvec) as [[ctrpc ctr] | ] eqn:LOOKUP;
 
     [
       (* Cache hit case *)
@@ -312,7 +427,7 @@ Ltac analyze_step :=
         )
       | solve_refine_state ] ]
       || let op := current_instr_opcode in fail 3 "failed miss case" op
-    ]
+    ]*)
   | _ : Symbolic.run_syscall _ _ = Some _ |- _ => idtac
   end.
 
@@ -323,20 +438,40 @@ Lemma forward_simulation sst sst' cst :
     exec (Concrete.step _ masks) cst cst' /\
     refine_state ki table sst' cst'.
 Proof.
-  intros REF STEP.
-  destruct REF as [smem sregs int cmem cregs cache epc pc tpc
-                   ? ? REFM REFR CACHE MVEC WFENTRYPOINTS KINV].
-  subst sst cst.
+  move=> REF STEP.
   inv STEP;
-  try match goal with
-  | H : Symbolic.State _ _ _ _ = Symbolic.State _ _ _ _ |- _ =>
-    inv H
-  end;
   match_data;
   repeat autounfold in NEXT;
-  match_inv;
+  match_inv.
 
   analyze_step.
+
+  concretize_ivec.
+
+  rewrite /build_cmvec.
+
+  eexists. split.
+  apply exec_one. solve_concrete_step.
+
+  econstructor; eauto; simpl.
+
+  assert (build_ivec table (Symbolic.State mem reg pc0@tpc0 extra) = Some mvec).
+  by rewrite /build_ivec; find_and_rewrite.
+  match goal with
+  | H : Concrete.cache_lookup _ _ ?cmvec = _ |- _ =>
+    assert (build_cmvec (Concrete.mkState cmem cregs cache pc0@tpc epc) = Some cmvec)
+  end.
+  by rewrite /build_cmvec; find_and_rewrite.
+
+
+
+  simpl.
+
+
+  let cmvec := concretize_ivec in
+  set (A := cmvec).
+
+  Focus 2.
 
   match goal with
     | |- context[exec _ ?cst _] =>
